Adapted code in acai/ to go through without module cloning/instantiation.

proofs/acai/XMSS_TW.ec
@@ -81,6 +81,7 @@ op [lossless full uniform] dmkey : mkey distr.
 (* PRF that generates indexing keys for message compression given a seed and an index *)  
 op mkg : mseed -> index -> mkey.
 
+(*
 clone import KeyedHashFunctions as MKG with
   type key_t <- mseed,
   type in_t <- index,
@@ -96,13 +97,14 @@ clone import PRF as MKG_PRF with
   
   proof *.
   realize dkey_ll by exact: dmseed_ll.
-  realize doutm_ll. by move=> _; apply dmkey_ll. qed.
+  realize doutm_ll by move=> _; apply dmkey_ll.
 
-
+*)
 
 (* --- Clones and imports --- *)
 (* -- Model -- *)
 (* Random oracle *)
+(*
 clone import ROM as MCORO with
   type in_t <- mkey * msgXMSSTW,
   type out_t <- msgFLXMSSTW,
@@ -118,9 +120,10 @@ clone import MCORO.LazyEager as MCOROLE with
   proof *. 
 
 module MCO = ERO.
-
+*)
 
 (* -- Scheme specification and security notions -- *)
+(*
 (* XMSS-TW (where the message compression function is considered to be an RO) *)
 clone import DigitalSignaturesROM as XMSSTW_ROM with
   type pk_t <- pkXMSSTW,
@@ -133,16 +136,10 @@ clone import DigitalSignaturesROM as XMSSTW_ROM with
   type d_in_t <- int,
   type d_out_t <- bool,
   
-    op doutm <- fun _ => dmsgFLXMSSTW,
-   
-  theory RO <- MCORO
+    op doutm <- fun _ => dmsgFLXMSSTW
   
   proof *.
-
-import XMSSTW_ROM.KeyUpdatingROM.
-import DSS.
-import KeyUpdating.
-
+*)
 
 (* -- Proof-specific -- *)
 (* Hash-then-sign proof technique *)
@@ -168,7 +165,8 @@ clone import HashThenSign as HtS with
     op WithPRF.dms <= dmseed,
     
   theory RCO <= MKey,
-  theory MSG_AL <= MsgXMSSTW,
+  theory MSG_AL <= MsgXMSSTW
+(*
   theory MCORO <= MCORO,
   theory MCOROLE <= MCOROLE,
   theory DSS_FL <= FLXMSSTW,
@@ -176,6 +174,7 @@ clone import HashThenSign as HtS with
   theory WithPRF.MKG <= MKG,
   theory WithPRF.MKG_PRF <= MKG_PRF,
   theory WithPRF.DSS_AL_PRF <= XMSSTW_ROM
+*)
   
   proof *.
   realize ge0_n by smt(ge2_l).
@@ -189,10 +188,11 @@ clone import HashThenSign as HtS with
   realize drco_fu by exact: dmkey_fu.
   realize WithPRF.dms_ll by exact: dmseed_ll.
 
-import WithPRF.
+import Repro MCORO MCOROLE.
+import EUFRMAEqv DSS_FL DSS_FL_EUFRMA.
+import WithPRF MKG MKG_PRF DSS_AL_PRF KeyUpdatingROM DSS KeyUpdating.
 import WS.
-import EUFRMAEqv.
-  
+
 
 (* --- XMSS-TW --- *)
 (* Specification of XMSS-TW (assuming the message compression function is an RO) *)
@@ -339,7 +339,9 @@ declare axiom A_forge_queries (RO <: POracle{-A, -QC_A}) (SO <: SOracle_CMA{-A, 
   hoare[A(QC_A(A, RO, SO).QC_RO, QC_A(A, RO, SO).QC_SO).forge : 
     QC_A.cH = 0 /\ QC_A.cS = 0 ==> QC_A.cH <= qH /\ QC_A.cS <= qS].
 
-
+print EUF_CMA_RO.
+print ALKUDSS_EUFCMARO_PRF_CRRO_EUFRMA.
+locate ALKUDSS_EUFCMARO_PRF_CRRO_EUFRMA.
 (* -- Security theorems -- *)
 (* 
   High-level security theorem (based on EUF-RMA of FL-XMSS-TW):
@@ -455,7 +457,12 @@ lemma EUFCMARO_XMSSTW &m :
   +
   l%r * mu1 dmsgFLXMSSTW witness.
 proof.
-move: (EUFRMA_FLXMSSTW (R_EUFRMA_IEUFRMA(R_EUFCMARO_IEUFRMA(A))) _ &m) (EUFCMARO_XMSSTW_EUFRMA &m); 2: smt().
+move: (EUFRMA_FLXMSSTW (R_EUFRMA_IEUFRMA(R_EUFCMARO_IEUFRMA(A))) _ &m) (EUFCMARO_XMSSTW_EUFRMA &m); last first.
+have -> /#:
+  Pr[FLXMSSTW_EUFRMA.EUF_RMA(FL_XMSS_TW, R_EUFRMA_IEUFRMA(R_EUFCMARO_IEUFRMA(A))).main() @ &m : res]
+  =
+  Pr[EUF_RMA(FL_XMSS_TW, R_EUFRMA_IEUFRMA(R_EUFCMARO_IEUFRMA(A))).main() @ &m : res].
++ by byequiv => //; sim.
 proc; inline *.
 wp; call (: true). 
 + by move=> RO SO ROll SOll; apply (A_forge_ll RO SO).
